

- Diffusion eqn (Find a Fourier series solution)

$$\frac{\partial u}{\partial t} = D \frac{\partial^2 u}{\partial x^2} \quad , \quad u(0,t) = 0 = u(l,t) \quad , \quad u(x,0) = f(x)$$

- Separation of variables  $u(x,t) = M(x)N(t)$

$$MN_t = D M_{xx} N$$

$$\frac{N_t}{N} = \frac{M_{xx}}{M} = -\lambda \quad , \quad \lambda \geq 0$$

$$\frac{\partial N}{\partial t} + \lambda N = 0 \quad , \quad \frac{\partial^2 M}{\partial x^2} + \lambda M = 0$$

$$\text{B.C.} \quad M(0)N = 0 = M(l)N \quad \Rightarrow \quad M(0) = 0 = M(l)$$

with solution

$$\lambda_k = \left(\frac{k\pi}{l}\right)^2 \quad , \quad M_k(x) = \sqrt{\frac{2}{l}} \sin\left(\frac{k\pi x}{l}\right) \quad , \quad k = 1, 2, 3, \dots$$

↓ (don't want  $k=0$  since it generates the trivial soln.)

$$N_k(t) = A_k e^{-D\left(\frac{k\pi}{l}\right)^2 t}$$

$$\therefore u_k(x,t) = A_k e^{-D\left(\frac{k\pi}{l}\right)^2 t} \sqrt{\frac{2}{l}} \sin\left(\frac{k\pi x}{l}\right)$$

Now to find the general soln.

$$u(x,t) = \sum_{k=1}^{\infty} A_k e^{-D\left(\frac{k\pi}{l}\right)^2 t} \sqrt{\frac{2}{l}} \sin\left(\frac{k\pi x}{l}\right)$$

impose  $u(x,0) = f(x)$

$$\sum_{k=1}^{\infty} A_k \cdot \underbrace{\sqrt{\frac{2}{l}} \sin\left(\frac{k\pi x}{l}\right)}_{M_k(x)} = f(x)$$

$$A_k = (f, M_k)$$

pick out the  $A_k$  for each term

note: as  $t \rightarrow \infty$ ,  $u \rightarrow 0$  for all  $f(x)$   
but the larger  $k$  terms decay faster!

- what if  $u(0,t) = 0$ ,  $u(l,t) = 1$

we would get  $M(l)N = 1$  if we do the same as before!

Consider : steady solution of  $\uparrow$  ( $\frac{\partial}{\partial t} \rightarrow 0$ )

$$D \frac{d^2 u}{dx^2} = 0 \quad , \quad u(0) = 0, \quad u(l) = 1$$

$$\hookrightarrow u(x) = Ax + B \quad \Rightarrow \quad u(x) = \frac{x}{l}$$

If we decompose  $u(x,t) = u(x) + \hat{u}(x,t)$ , what determines  $\hat{u}(x,t)$ ?

$$\text{but since } \frac{\partial u}{\partial t} = 0 = \frac{\partial^2 u}{\partial x^2} \quad , \quad \underbrace{\frac{\partial \hat{u}}{\partial t} = D \frac{\partial^2 \hat{u}}{\partial x^2}}_{\text{still the same PDE.}}$$

$$u(0,t) = 0 = \overset{=0}{u(0)} + \hat{u}(0,t) \Rightarrow \hat{u}(0,t) = 0$$

$$u(l,t) = 1 = \overset{=1}{u(l)} + \hat{u}(l,t) \Rightarrow \hat{u}(l,t) = 0$$

$$\text{IC: } u(x,0) = f(x) = \frac{x}{l} + \hat{u}(x,0) \Rightarrow \hat{u}(x,0) = f - \frac{x}{l} = \hat{f}(x)$$

the solution to  $\hat{u}$  is the same as before, just with different IC!

The solution as  $t \rightarrow \infty$  is just the steady state solution  $u$